Tests/TestTag.lean
@@ -40,3 +40,33 @@ info: 0
 -/
 #guard_msgs in
 #eval barB.offset
+
+/--
+error: Only functions of type ℕ → ℕ or ℕ → ℤ are supported
+-/
+#guard_msgs in
+/--
+goo
+-/
+@[OEIS := A0010]
+def goo (n : Nat) : Rat := n
+
+/--
+error: Only functions of type ℕ → ℕ or ℕ → ℤ are supported
+-/
+#guard_msgs in
+/--
+spam
+-/
+@[OEIS := A005]
+def spam : Nat → Rat → Rat  := fun m n => n + m
+
+/--
+error: Only functions of type ℕ → ℕ or ℕ → ℤ are supported
+-/
+#guard_msgs in
+/--
+baz2
+-/
+@[OEIS := A006]
+theorem baz2 (n : Nat) : n ≤ n := Nat.le_refl n
